wip

src/drf/AbortProp.v
@@ -35,16 +35,326 @@ Require Import PredStep.
 Set Implicit Arguments.
 
 
-Inductive added_memory (tm: TimeMap.t): Memory.t -> Memory.t -> Prop :=
-| added_memory_intro
-    m0 loc to from msg m1
-    (TLE: Time.le (tm loc) to) 
-    (ADD: Memory.add m0 loc to from msg m1)
+
+Inductive added_memory_imm (tm: TimeMap.t): Memory.t -> Memory.t -> Prop :=
+| added_memory_imm_intro
+    m0 loc to from val m1
+    (TLE: Time.le (tm loc) to)
+    (ADD: Memory.add m0 loc to from (Message.full val None) m1)
   :
-    added_memory tm m0 m1
+    added_memory_imm tm m0 m1
 .
 
-(* Lemma thread_consistent_no_sc_no_acq *)
+Definition added_memory (tm: TimeMap.t) := rtc (added_memory_imm tm).
+
+Lemma added_memory_future tm m0 m1
+      (ADDED: added_memory tm m0 m1)
+  :
+    Memory.future m0 m1.
+Proof.
+  ginduction ADDED; auto. etrans; [| apply IHADDED].
+  inv H. econs; eauto. econs; eauto.
+  econs. ss. eapply Time.bot_spec.
+Qed.
+
+Definition is_cancel (e: ThreadEvent.t) : Prop :=
+  match e with
+  | ThreadEvent.promise _ _ _ _ Memory.op_kind_cancel => True
+  | _ => False
+  end.
+
+Inductive only_reserves (proms: Memory.t): Prop :=
+| only_reserves_intro
+    (RESERVES: forall loc to from msg (GET: Memory.get loc to proms = Some (from, msg)),
+        msg = Message.reserve)
+    (FINITE: Memory.finite proms)
+.
+
+Lemma reserves_cancelable lang st vw proms sc mem0
+      (RESERVES: only_reserves proms)
+      (MLE: Memory.le proms mem0)
+  :
+    exists mem1,
+      rtc (tau (@pred_step is_cancel lang))
+          (Thread.mk lang st (Local.mk vw proms) sc mem0)
+          (Thread.mk lang st (Local.mk vw Memory.bot) sc mem1).
+Proof.
+  inv RESERVES. unfold Memory.finite in *. des.
+  ginduction dom; ss; i.
+  - exists mem0. replace proms with Memory.bot; auto.
+    eapply Memory.ext. i. rewrite Memory.bot_get.
+    destruct (Memory.get loc ts proms) as [[from msg]|] eqn:GET; auto.
+    exfalso. eauto.
+  - destruct a as [loc' to'].
+    destruct (Memory.get loc' to' proms) as [[from' msg']|] eqn:GET.
+    + exploit RESERVES0; eauto. i. clarify.
+      exploit Memory.remove_exists.
+      { eapply GET. }
+      intros [prom1 REMOVE0].
+      exploit Memory.remove_exists.
+      { eapply MLE. eapply GET. }
+      intros [mem1 REMOVE1]. hexploit IHdom.
+      * instantiate (1:=mem1). instantiate (1:=prom1).
+        ii. erewrite Memory.remove_o in LHS; eauto. des_ifs.
+        eapply MLE in LHS. erewrite Memory.remove_o; eauto. des_ifs.
+        ss. des; clarify.
+      * i. erewrite Memory.remove_o in GET0; eauto. des_ifs.
+        eapply RESERVES0; eauto.
+      * i. erewrite Memory.remove_o in GET0; eauto. des_ifs.
+        exploit FINITE; eauto. i. ss.
+        des; ss; clarify.
+      * i. des. exists mem2. econs 2.
+        { econs.
+          - instantiate (2:=ThreadEvent.promise loc' from' to' Message.reserve Memory.op_kind_cancel).
+            econs; ss. econs. econs 1. econs; ss.
+            econs; ss. econs; eauto.
+          - ss. }
+        eapply H.
+    + eapply IHdom; eauto.
+      i. exploit FINITE; eauto. i. des; clarify.
+Qed.
+
+Inductive lower_memory (mem_src mem_tgt: Memory.t): Prop :=
+| lower_memory_intro
+    (COVER: forall loc to (COV: covered loc to mem_src),
+        covered loc to mem_tgt)
+    (MLE: forall loc to from_tgt vw_tgt val
+                 (GETTGT: Memory.get loc to mem_tgt = Some (from_tgt, Message.full val vw_tgt)),
+        exists from_src vw_src,
+          (<<GETSRC: Memory.get loc to mem_src = Some (from_src, Message.full val vw_src)>>) /\
+          (<<VWLE: View.opt_le vw_src vw_tgt>>)).
+
+
+Inductive lower_event: ThreadEvent.t -> ThreadEvent.t -> Prop :=
+| lower_event_silent:
+    lower_event ThreadEvent.silent ThreadEvent.silent
+| lower_event_syscall e:
+    lower_event (ThreadEvent.syscall e) (ThreadEvent.syscall e)
+| lower_event_failure:
+    lower_event ThreadEvent.failure ThreadEvent.failure
+| lower_event_fence ordr ordw:
+    lower_event (ThreadEvent.fence ordr ordw) (ThreadEvent.fence ordr ordw)
+| lower_event_read
+    loc to val vw_src vw_tgt ordr
+    (VWLE: View.opt_le vw_src vw_tgt)
+  :
+    lower_event
+      (ThreadEvent.read loc to val vw_src ordr)
+      (ThreadEvent.read loc to val vw_tgt ordr)
+| lower_event_write
+    loc from to val vw_src vw_tgt ordw
+    (VWLE: View.opt_le vw_src vw_tgt)
+  :
+    lower_event
+      (ThreadEvent.write loc from to val vw_src ordw)
+      (ThreadEvent.write loc from to val vw_tgt ordw)
+| lower_event_update
+    loc from to valr valw vwr_src vwr_tgt vww_src vww_tgt ordr ordw
+    (VWRLE: View.opt_le vwr_src vwr_tgt)
+    (VWWLE: View.opt_le vww_src vww_tgt)
+  :
+    lower_event
+      (ThreadEvent.update loc from to valr valw vwr_src vww_src ordr ordw)
+      (ThreadEvent.update loc from to valr valw vwr_tgt vww_tgt ordr ordw)
+| lower_event_promise
+    loc from to msg kind
+  :
+    lower_event
+      (ThreadEvent.promise loc from to msg kind)
+      (ThreadEvent.promise loc from to msg kind)
+.
+Hint Constructors lower_event.
+
+Lemma lower_memory_closed_message msg mem_src mem_tgt
+      (LOWMEM: lower_memory mem_src mem_tgt)
+      (CLOSED: Memory.closed_message msg mem_tgt)
+  :
+    Memory.closed_message msg mem_src.
+Proof.
+  inv CLOSED; eauto. inv CLOSED0; eauto. econs. econs.
+  inv CLOSED. inv LOWMEM. econs.
+  - ii. specialize (PLN loc). des.
+    eapply MLE in PLN. des. esplits; eauto.
+  - ii. specialize (RLX loc). des.
+    eapply MLE in RLX. des. esplits; eauto.
+Qed.
+
+Lemma promise_consistent_mon v_src v_tgt prom
+      (CONSISTENT: Local.promise_consistent (Local.mk v_tgt prom))
+      (VWLE: TView.le v_src v_tgt)
+  :
+    Local.promise_consistent (Local.mk v_src prom).
+Proof.
+  ii. ss. exploit CONSISTENT; eauto. i. ss.
+  eapply TimeFacts.le_lt_lt; eauto. eapply VWLE.
+Qed.
+
+Lemma lower_memory_promise mem_src0 mem_tgt0 prom0
+      loc from to msg prom1 mem_tgt1 kind
+      (LOWMEM: lower_memory mem_src0 mem_tgt0)
+      (MLESRC: Memory.le prom0 mem_src0)
+      (MLETGT: Memory.le prom0 mem_tgt0)
+      (PROMISE: Memory.promise prom0 mem_tgt0 loc from to msg prom1 mem_tgt1 kind)
+  :
+    exists mem_src1,
+      (<<PROMISE: Memory.promise prom0 mem_src0 loc from to msg prom1 mem_src1 kind>>) /\
+      (<<LOWMEM: lower_memory mem_src1 mem_tgt1>>).
+Proof.
+Admitted.
+
+Lemma lower_memory_write mem_src0 mem_tgt0 prom0
+      loc from to val vw_src vw_tgt prom1 mem_tgt1 kind
+      (LOWMEM: lower_memory mem_src0 mem_tgt0)
+      (MLESRC: Memory.le prom0 mem_src0)
+      (MLETGT: Memory.le prom0 mem_tgt0)
+      (VWLE: View.opt_le vw_src vw_tgt)
+      (VWWF: View.opt_wf vw_src)
+      (PROMISE: Memory.write prom0 mem_tgt0 loc from to val vw_tgt prom1 mem_tgt1 kind)
+  :
+    exists mem_src1,
+      (<<PROMISE: Memory.write prom0 mem_src0 loc from to val vw_src prom1 mem_src1 kind>>) /\
+      (<<LOWMEM: lower_memory mem_src1 mem_tgt1>>).
+Proof.
+Admitted.
+
+Lemma tview_read_fence_wf
+      ord tview
+      (WF_TVIEW: TView.wf tview)
+  :
+    TView.wf (TView.read_fence_tview tview ord).
+Proof.
+  econs; ss; eauto.
+  - i. eapply WF_TVIEW.
+  - des_ifs; eapply WF_TVIEW.
+  - eapply WF_TVIEW.
+  - i. des_ifs; try eapply WF_TVIEW.
+    etrans; eapply WF_TVIEW.
+  - des_ifs; try eapply WF_TVIEW. refl.
+Qed.
+
+Lemma lower_memory_step
+      lang prom th_src th_tgt th_tgt' st st' v_src v_tgt v_tgt' prom' sc_src sc_tgt sc_tgt'
+      mem_src mem_tgt mem_tgt' tf e_tgt
+      (VWFSRC: TView.wf v_src)
+      (VWFTGT: TView.wf v_tgt)
+      (VIEW: TView.le v_src v_tgt)
+      (SC: TimeMap.le sc_src sc_tgt)
+      (TH_SRC: th_src = Thread.mk lang st (Local.mk v_src prom) sc_src mem_src)
+      (TH_TGT0: th_tgt = Thread.mk lang st (Local.mk v_tgt prom) sc_tgt mem_tgt)
+      (TH_TGT1: th_tgt' = Thread.mk lang st' (Local.mk v_tgt' prom') sc_tgt' mem_tgt')
+      (LOWMEM: lower_memory mem_src mem_tgt)
+      (MLESRC: Memory.le prom mem_src)
+      (MLETGT: Memory.le prom mem_tgt)
+      (STEP: Thread.step tf e_tgt th_tgt th_tgt')
+  :
+    exists e_src v_src' mem_src' sc_src',
+      (<<STEP: Thread.step
+                 tf e_src th_src
+                 (Thread.mk lang st' (Local.mk v_src' prom') sc_src' mem_src')>>) /\
+      (<<VIEW: TView.le v_src' v_tgt'>>) /\
+      (<<LOWMEM: lower_memory mem_src' mem_tgt'>>) /\
+      (<<EVT: lower_event e_src e_tgt>>) /\
+      (<<SC: TimeMap.le sc_src' sc_tgt'>>)
+.
+Proof.
+  clarify. inv STEP.
+  - inv STEP0. inv LOCAL. clarify. ss.
+    exploit lower_memory_promise; eauto. i. des. esplits; eauto.
+    econs; eauto. econs 1; eauto. econs; eauto.
+    eapply lower_memory_closed_message; eauto.
+  - inv STEP0. inv LOCAL.
+    + exists ThreadEvent.silent. esplits; eauto.
+      econs 2; eauto. econs; eauto.
+    + inv LOCAL0. ss. clarify. dup LOWMEM. inv LOWMEM.
+      exploit MLE; eauto. i. des.
+      exists (ThreadEvent.read loc ts val vw_src ord). esplits; eauto.
+      * econs 2; eauto. econs; eauto. econs; eauto. econs; eauto. ss.
+        eapply TViewFacts.readable_mon; eauto.
+        { inv VIEW. eauto. }
+        { refl. }
+      * ss. eapply TViewFacts.read_tview_mon; eauto.
+        { eapply Cell.get_opt_wf in GET. inv GET. eauto. }
+        { refl. }
+    + inv LOCAL0. ss. clarify.
+      assert (RELEASEDLE:
+                View.opt_le
+                  (TView.write_released v_src sc_src loc to None ord)
+                  (TView.write_released v_tgt sc_tgt loc to None ord)).
+      { eapply TViewFacts.write_released_mon; eauto. refl. }
+      exploit lower_memory_write; eauto.
+      { eapply TViewFacts.write_future0; eauto. } i. des.
+      dup LOWMEM. inv LOWMEM.
+      exists (ThreadEvent.write loc from to val (TView.write_released v_src sc_src loc to None ord) ord).
+      esplits; eauto.
+      * econs 2; eauto. econs; eauto. econs; eauto. econs; eauto. ss.
+        eapply TViewFacts.writable_mon; eauto.
+        { inv VIEW. eauto. }
+        { refl. }
+      * ss. eapply TViewFacts.write_tview_mon; eauto. refl.
+    + inv LOCAL1. inv LOCAL2. ss. clarify.
+      dup LOWMEM. inv LOWMEM.
+      exploit MLE; eauto. i. des.
+      exists (ThreadEvent.update
+                loc tsr tsw valr valw vw_src
+                (TView.write_released (TView.read_tview v_src loc tsr vw_src ordr) sc_src loc tsw
+                                      vw_src ordw) ordr ordw).
+      assert (RELEASEDLE: View.opt_le
+                            (TView.write_released (TView.read_tview v_src loc tsr vw_src ordr) sc_src loc tsw vw_src ordw)
+                            (TView.write_released (TView.read_tview v_tgt loc tsr releasedr ordr) sc_tgt loc tsw
+                                                  releasedr ordw)).
+      { dup GET. eapply Cell.get_opt_wf in GET. inv GET.
+        eapply TViewFacts.write_released_mon; try eassumption.
+        - eapply TViewFacts.read_tview_mon; eauto. refl.
+        - eapply TViewFacts.read_future1; eauto.
+        - refl. }
+      exploit lower_memory_write; try apply WRITE; try eassumption.
+      { dup GETSRC. eapply Cell.get_opt_wf in GETSRC. inv GETSRC.
+        ss. eapply TViewFacts.write_future0; eauto.
+        eapply TViewFacts.read_future1; eauto. }
+      i. des.
+      esplits; eauto.
+      * econs 2; eauto. econs; eauto. econs; eauto.
+        { econs; eauto. ss.
+          eapply TViewFacts.readable_mon; eauto.
+          - eapply VIEW; eauto.
+          - refl. }
+        { econs; eauto. ss.
+          eapply TViewFacts.writable_mon; eauto.
+          - eapply View.join_le.
+            + eapply View.join_le; eauto.
+              * eapply VIEW.
+              * refl.
+            + des_ifs.
+              * eapply View.unwrap_opt_le; eauto.
+              * refl.
+          - refl. }
+      * ss. eapply TViewFacts.write_tview_mon; eauto.
+        { eapply TViewFacts.read_tview_mon; eauto.
+          - dup GET. eapply Cell.get_opt_wf in GET. inv GET. eauto.
+          - refl. }
+        { eapply TViewFacts.read_future1; eauto.
+          dup GET. eapply Cell.get_opt_wf in GET. inv GET. eauto. }
+        { refl. }
+    + inv LOCAL0. ss. clarify. esplits; eauto.
+      * econs 2; eauto. econs; eauto.
+      * ss. eapply TViewFacts.write_fence_tview_mon; eauto.
+        { eapply TViewFacts.read_fence_tview_mon; eauto. refl. }
+        { refl. }
+        { eapply tview_read_fence_wf; eauto. }
+      * ss. eapply TViewFacts.write_fence_sc_mon; eauto.
+        { eapply TViewFacts.read_fence_tview_mon; eauto. refl. }
+        { refl. }
+    + inv LOCAL0. ss. clarify. esplits; eauto.
+      * econs 2; eauto. econs; eauto.
+      * ss. eapply TViewFacts.write_fence_tview_mon; eauto.
+        { eapply TViewFacts.read_fence_tview_mon; eauto. }
+        { eapply tview_read_fence_wf; eauto. }
+      * ss. eapply TViewFacts.write_fence_sc_mon; eauto.
+        { eapply TViewFacts.read_fence_tview_mon; eauto. }
+    + inv LOCAL0. ss. clarify. esplits; eauto.
+      * econs 2; eauto. econs; eauto. econs; eauto.
+        econs; eauto. eapply promise_consistent_mon; eauto.
+Qed.
 
 Lemma progressable_in_added_rtc
       lang st lc sc0 sc1 m0 m1 tm
@@ -57,4 +367,98 @@ Lemma progressable_in_added_rtc
                     (Thread.mk _ st lc sc1 m1) e2>>) /\
       (<<PROMISES: Local.promises (Thread.local e2) = Memory.bot>>).
 Proof.
+Admitted.
+
+Definition same_locs_memory (L: Loc.t -> Prop) (mem_src mem_tgt: Memory.t): Prop :=
+  forall loc (SAT: L loc) to,
+    Memory.get loc to mem_src = Memory.get loc to mem_tgt.
+
+Definition locs_in (L: Loc.t -> Prop) (e : ThreadEvent.t) : Prop :=
+  match e with
+  | ThreadEvent.promise loc _ _ _ _ => L loc
+  | ThreadEvent.read loc _ _ _ _ => L loc
+  | ThreadEvent.write loc _ _ _ _ _ => L loc
+  | ThreadEvent.update loc _ _ _ _ _ _ _ _=> L loc
+  | _ => True
+  end.
+
+Lemma same_locs_memory_remove L mem_src0 mem_tgt0
+      loc from to msg mem_tgt1
+      (SAMELOCS: same_locs_memory L mem_src0 mem_tgt0)
+      (REMOVE: Memory.remove mem_tgt0 loc from to msg mem_tgt1)
+      (SAT: L loc)
+  :
+    exists mem_src1,
+      (<<REMOVE: Memory.remove mem_src0 loc from to msg mem_src1>>) /\
+      (<<SAMELOCS: same_locs_memory L mem_src1 mem_tgt1>>).
+Proof.
+  exploit Memory.remove_get0; eauto. i. des.
+  exploit Memory.remove_exists.
+  - erewrite SAMELOCS; eauto.
+  - i. des. esplits; eauto.
+    ii. erewrite (@Memory.remove_o mem2); eauto.
+    erewrite (@Memory.remove_o mem_tgt1); cycle 1; eauto.
+    des_ifs. eapply SAMELOCS; eauto.
+Qed.
+
+Lemma same_locs_memory_promise L mem_src0 mem_tgt0 prom0
+      loc from to msg prom1 mem_tgt1 kind
+      (SAMELOCS: same_locs_memory L mem_src0 mem_tgt0)
+      (PROMISE: Memory.promise prom0 mem_tgt0 loc from to msg prom1 mem_tgt1 kind)
+      (SAT: L loc)
+  :
+    exists mem_src1,
+      (<<PROMISE: Memory.promise prom0 mem_src0 loc from to msg prom1 mem_src1 kind>>) /\
+      (<<SAMELOCS: same_locs_memory L mem_src1 mem_tgt1>>).
+Proof.
+  inv PROMISE.
+  - dup MEM. inv MEM0. inv ADD.
+    exploit Memory.add_exists.
+    + instantiate (1:=to). instantiate (1:=from).
+      instantiate (1:=mem_src0). instantiate (1:=loc).
+      ii. exploit SAMELOCS; eauto.
+      unfold Memory.get, Cell.get. i.
+      eapply DISJOINT; eauto. erewrite <- x0. eauto.
+    + eauto.
+    + eauto.
+    + i. des. exists mem2. esplits; eauto.
+      * econs 1; eauto. i.
+Admitted.
+
+Lemma same_locs_memory_write L mem_src0 mem_tgt0 prom0
+      loc from to val vw prom1 mem_tgt1 kind
+      (SAMELOCS: same_locs_memory L mem_src0 mem_tgt0)
+      (PROMISE: Memory.write prom0 mem_tgt0 loc from to val vw prom1 mem_tgt1 kind)
+      (SAT: L loc)
+  :
+    exists mem_src1,
+      (<<PROMISE: Memory.write prom0 mem_src0 loc from to val vw prom1 mem_src1 kind>>) /\
+      (<<SAMELOCS: same_locs_memory L mem_src1 mem_tgt1>>).
+Proof.
+  inv PROMISE. exploit same_locs_memory_promise; eauto. i. des.
+  esplits; eauto.
+Qed.
+
+Lemma same_locs_memory_step
+      L lang prom th_src th_tgt th_tgt' st st' v v' prom' sc sc'
+      mem_src mem_tgt mem_tgt' tf e
+      (TH_SRC: th_src = Thread.mk lang st (Local.mk v prom) sc mem_src)
+      (TH_TGT0: th_tgt = Thread.mk lang st (Local.mk v prom) sc mem_tgt)
+      (TH_TGT1: th_tgt' = Thread.mk lang st' (Local.mk v' prom') sc' mem_tgt')
+      (SAMELOCS: same_locs_memory L mem_src mem_tgt)
+      (STEP: pred_step (locs_in L) e th_tgt th_tgt')
+  :
+    exists mem_src',
+      (<<STEP: Thread.step
+                 tf e th_src
+                 (Thread.mk lang st' (Local.mk v' prom') sc' mem_src')>>) /\
+      (<<SAMELOCS: same_locs_memory L mem_src' mem_tgt' >>)
+.
+Proof.
+  clarify. inv STEP. inv STEP0. inv STEP.
+  - inv STEP0. inv LOCAL. ss. clarify.
+    exploit same_locs_memory_promise; eauto. i. des.
+    exists mem_src1. esplits; eauto.
+    econs 1; eauto. econs; eauto.
+    + econs; eauto. eauto.
 Admitted.
